Automate equivariance for almost all uses of binder_inductive
The only one missing is InfFOL, because one of the existentials needs to
be instantiated with a subst function which needs pre- and
post-composition with the permutation.

thys/Pi_Calculus/Pi_cong.thy
@@ -2,12 +2,6 @@ theory Pi_cong
   imports Commitment
 begin
 
-abbreviation Tsupp :: "trm \<Rightarrow> trm \<Rightarrow> var set" where
-  "Tsupp e1 e2 \<equiv> FFVars e1 \<union> FFVars e2"
-
-lemma fresh: "\<exists>xx. xx \<notin> Tsupp (t :: trm) t2"
-  by (metis (no_types, lifting) exists_var finite_iff_le_card_var term.Un_bound term.set_bd_UNIV)
-
 (* Structural congurence *)
 inductive cong :: "trm \<Rightarrow> trm \<Rightarrow> bool" (infix "(\<equiv>\<^sub>\<pi>)" 40) where
   "P = Q \<Longrightarrow> P \<equiv>\<^sub>\<pi> Q"
@@ -17,15 +11,9 @@ inductive cong :: "trm \<Rightarrow> trm \<Rightarrow> bool" (infix "(\<equiv>\<
 | "x \<noteq> y \<Longrightarrow> Res x (Res y P) \<equiv>\<^sub>\<pi> Res y (Res x P)"
 | "Res x Zero \<equiv>\<^sub>\<pi> Zero"
 | "Bang P \<equiv>\<^sub>\<pi> Par P (Bang P)"
-| cong_3: "x \<notin> FFVars Q \<Longrightarrow> Res x (Par P Q) \<equiv>\<^sub>\<pi> Par (Res x P) Q"
+| "x \<notin> FFVars Q \<Longrightarrow> Res x (Par P Q) \<equiv>\<^sub>\<pi> Par (Res x P) Q"
 
 binder_inductive cong
-  subgoal for R B \<sigma> x1 x2
-    apply simp
-    by (elim disj_forward case_prodE)
-      (auto simp: isPerm_def term.permute_comp bij_implies_inject
-        | ((rule exI[of _ "\<sigma> _"] exI)+, (rule conjI)?, rule refl)
-        | ((rule exI[of _ "\<sigma> _"])+; auto))+
   subgoal premises prems for R B P Q
     by (tactic \<open>refreshability_tac false
       [@{term "FFVars :: trm \<Rightarrow> var set"}, @{term "FFVars :: trm \<Rightarrow> var set"}]
@@ -40,20 +28,6 @@ binder_inductive cong
 thm cong.strong_induct
 thm cong.equiv
 
-lemma finite_Tsupp: "finite (Tsupp x1 x2)"
-  by (metis commit.set(4) finite_FVars_commit finite_Un)
-
-lemma exists_fresh:
-  "\<exists> z. z \<notin> set xs \<and> (z \<notin> Tsupp x1 x2)"
-proof-
-  have 0: "|set xs \<union> Tsupp x1 x2| <o |UNIV::var set|"
-    unfolding ls_UNIV_iff_finite
-    using finite_Tsupp by blast
-  then obtain x where "x \<notin> set xs \<union> Tsupp x1 x2"
-    using MRBNF_FP.exists_fresh by blast
-  thus ?thesis by auto
-qed
-
 inductive trans :: "trm \<Rightarrow> trm \<Rightarrow> bool" (infix "(\<rightarrow>)" 30) where
   "Par (Out x z P) (Inp x y Q) \<rightarrow> Par P (usub Q z y)"
 | "P \<rightarrow> Q \<Longrightarrow> Par P R \<rightarrow> Par P Q"
@@ -61,13 +35,6 @@ inductive trans :: "trm \<Rightarrow> trm \<Rightarrow> bool" (infix "(\<rightar
 | "P \<equiv>\<^sub>\<pi> P' \<Longrightarrow> P' \<rightarrow> Q' \<Longrightarrow> Q' \<equiv>\<^sub>\<pi> Q \<Longrightarrow> P \<rightarrow> Q"
 
 binder_inductive trans
-  subgoal for R B \<sigma> x1 x2
-    apply simp
-    apply (elim disj_forward exE)
-       apply  (auto simp: isPerm_def term.permute_comp
-        | ((rule exI[of _ "\<sigma> _"] exI)+, (rule conjI)?, rule refl)
-        | ((rule exI[of _ "\<sigma> _"])+; auto))+
-    by (metis cong.equiv bij_imp_inv' term.permute_bij term.permute_inv_simp)
   subgoal premises prems for R B P Q
     by (tactic \<open>refreshability_tac false
       [@{term "FFVars :: trm \<Rightarrow> var set"}, @{term "FFVars :: trm \<Rightarrow> var set"}]
