thys/MRBNF_Recursor.thy
@@ -17,6 +17,22 @@ lemma ex_forward'[equiv_forward 3]: "\<exists>x. P x \<Longrightarrow> (\<And>x.
   by blast
 declare conj_forward[equiv_forward] disj_forward[equiv_forward]
 
+declare inj_image_mem_iff[OF bij_is_inj, equiv]
+
+lemma image_Int_empty[equiv]: "bij f \<Longrightarrow> f ` A \<inter> f ` B = {} \<longleftrightarrow> A \<inter> B = {}"
+  by (metis bij_is_inj image_Int image_is_empty)
+lemma Un_equiv[equiv]: "bij f \<Longrightarrow> f ` (A \<union> B) = f ` A \<union> f ` B"
+  by (rule image_Un)
+lemma singleton_equiv[equiv]: "bij f \<Longrightarrow> f ` {x} = {f x}"
+  by simp
+lemma insert_equiv[equiv]: "bij f \<Longrightarrow> f ` insert x A = insert (f x) (f ` A)"
+  by (rule image_insert)
+lemma neq_equiv[equiv]: "bij f \<Longrightarrow> f a \<noteq> f b \<longleftrightarrow> a \<noteq> b"
+  by (simp add: bij_implies_inject)
+
+lemma notin_Un_forward: "x \<notin> A \<union> B \<Longrightarrow> (x \<notin> A \<Longrightarrow> y \<notin> C) \<Longrightarrow> (x \<notin> B \<Longrightarrow> y \<notin> D) \<Longrightarrow> y \<notin> C \<union> D"
+  by blast
+
 ML_file \<open>../Tools/mrbnf_vvsubst.ML\<close>
 
 ML_file \<open>../Tools/mrbnf_tvsubst.ML\<close>
